Locally Nameless Beta Confluence (#11)
* confluence

* non-terminal simps

* style

* use reduction_sys

* non-terminal simp

* remove redundant lemma

* update TODO

* style

* fix Trans instances

* use Trans instance for brevity

* add a reference

* para_lc_l and para_lc_r as

* naming conventions

* change confusing names

* aesop ruleset

* rm unused lemma

* ASCII arrows

* missed rule_sets

* use proof irrelevance

* style

* namespace rule set

Cslib/Computability/LambdaCalculus/Untyped/LocallyNameless/Basic.lean
@@ -6,6 +6,7 @@ Authors: Chris Henson
 
 import Cslib.Data.HasFresh
 import Cslib.Syntax.HasSubstitution
+import Cslib.Computability.LambdaCalculus.Untyped.LocallyNameless.AesopRuleset
 
 /-! # λ-calculus
 
@@ -36,9 +37,10 @@ inductive Term (Var : Type u)
 /-- Function application. -/
 | app  : Term Var → Term Var → Term Var
 
+namespace Term
+
 /-- Variable opening of the ith bound variable. -/
-@[simp]
-def Term.openRec (i : ℕ) (sub : Term Var) : Term Var → Term Var
+def openRec (i : ℕ) (sub : Term Var) : Term Var → Term Var
 | bvar i' => if i = i' then sub else bvar i'
 | fvar x  => fvar x
 | app l r => app (openRec i sub l) (openRec i sub r)
@@ -46,15 +48,25 @@ def Term.openRec (i : ℕ) (sub : Term Var) : Term Var → Term Var
 
 scoped notation:68 e "⟦" i " ↝ " sub "⟧"=> Term.openRec i sub e 
 
+@[aesop norm (rule_sets := [LambdaCalculus.LocallyNameless.ruleSet])]
+lemma openRec_bvar : (bvar i')⟦i ↝ s⟧ = if i = i' then s else bvar i' := by rfl
+
+@[aesop norm (rule_sets := [LambdaCalculus.LocallyNameless.ruleSet])]
+lemma openRec_fvar : (fvar x)⟦i ↝ s⟧ = fvar x := by rfl
+
+@[aesop norm (rule_sets := [LambdaCalculus.LocallyNameless.ruleSet])]
+lemma openRec_app : (app l r)⟦i ↝ s⟧ = app (l⟦i ↝ s⟧) (r⟦i ↝ s⟧) := by rfl
+
+@[aesop norm (rule_sets := [LambdaCalculus.LocallyNameless.ruleSet])]
+lemma openRec_abs : M.abs⟦i ↝ s⟧ = M⟦i + 1 ↝ s⟧.abs := by rfl
+
 /-- Variable opening of the closest binding. -/
-@[simp]
-def Term.open' {X} (e u):= @Term.openRec X 0 u e
+def open' {X} (e u):= @Term.openRec X 0 u e
 
 infixr:80 " ^ " => Term.open'
 
 /-- Variable closing, replacing a free `fvar x` with `bvar k` -/
-@[simp]
-def Term.closeRec (k : ℕ) (x : Var) : Term Var → Term Var
+def closeRec (k : ℕ) (x : Var) : Term Var → Term Var
 | fvar x' => if x = x' then bvar k else fvar x'
 | bvar i  => bvar i
 | app l r => app (closeRec k x l) (closeRec k x r)
@@ -62,15 +74,31 @@ def Term.closeRec (k : ℕ) (x : Var) : Term Var → Term Var
 
 scoped notation:68 e "⟦" k " ↜ " x "⟧"=> Term.closeRec k x e 
 
+variable {x : Var}
+
+omit [HasFresh Var] in
+@[aesop norm (rule_sets := [LambdaCalculus.LocallyNameless.ruleSet])]
+lemma closeRec_bvar : (bvar i)⟦k ↜ x⟧ = bvar i := by rfl
+
+omit [HasFresh Var] in
+@[aesop norm (rule_sets := [LambdaCalculus.LocallyNameless.ruleSet])]
+lemma closeRec_fvar : (fvar x')⟦k ↜ x⟧ = if x = x' then bvar k else fvar x' := by rfl
+
+omit [HasFresh Var] in
+@[aesop norm (rule_sets := [LambdaCalculus.LocallyNameless.ruleSet])]
+lemma closeRec_app : (app l r)⟦k ↜ x⟧ = app (l⟦k ↜ x⟧) (r⟦k ↜ x⟧) := by rfl
+
+omit [HasFresh Var] in
+@[aesop norm (rule_sets := [LambdaCalculus.LocallyNameless.ruleSet])]
+lemma closeRec_abs : t.abs⟦k ↜ x⟧ = t⟦k + 1 ↜ x⟧.abs := by rfl
+
 /-- Variable closing of the closest binding. -/
-@[simp]
-def Term.close {Var} [DecidableEq Var] (e u):= @Term.closeRec Var _ 0 u e
+def close {Var} [DecidableEq Var] (e u):= @Term.closeRec Var _ 0 u e
 
 infixr:80 " ^* " => Term.close
 
 /- Substitution of a free variable to a term. -/
-@[simp]
-def Term.subst (m : Term Var) (x : Var) (sub : Term Var) : Term Var :=
+def subst (m : Term Var) (x : Var) (sub : Term Var) : Term Var :=
   match m with
   | bvar i  => bvar i
   | fvar x' => if x = x' then sub else fvar x'
@@ -78,20 +106,40 @@ def Term.subst (m : Term Var) (x : Var) (sub : Term Var) : Term Var :=
   | abs M   => abs $ M.subst x sub
 
 /-- `Term.subst` is a substitution for λ-terms. Gives access to the notation `m[x := n]`. -/
-@[simp]
 instance instHasSubstitutionTerm : HasSubstitution (Term Var) Var where
   subst := Term.subst
 
+omit [HasFresh Var] in
+@[aesop norm (rule_sets := [LambdaCalculus.LocallyNameless.ruleSet])]
+lemma subst_bvar {n : Term Var} : (bvar i)[x := n] = bvar i := by rfl
+
+omit [HasFresh Var] in
+@[aesop norm (rule_sets := [LambdaCalculus.LocallyNameless.ruleSet])]
+lemma subst_fvar : (fvar x')[x := n] = if x = x' then n else fvar x' := by rfl
+
+omit [HasFresh Var] in
+@[aesop norm (rule_sets := [LambdaCalculus.LocallyNameless.ruleSet])]
+lemma subst_app {l r : Term Var} : (app l r)[x := n] = app (l[x := n]) (r[x := n]) := by rfl
+
+omit [HasFresh Var] in
+@[aesop norm (rule_sets := [LambdaCalculus.LocallyNameless.ruleSet])]
+lemma subst_abs {M : Term Var} : M.abs[x := n] = M[x := n].abs := by rfl
+
+omit [HasFresh Var] in
+@[aesop norm (rule_sets := [LambdaCalculus.LocallyNameless.ruleSet])]
+lemma subst_def (m : Term Var) (x : Var) (n : Term Var) : m.subst x n = m[x := n] := by rfl
+
 /-- Free variables of a term. -/
 @[simp]
-def Term.fv : Term Var → Finset Var
+def fv : Term Var → Finset Var
 | bvar _ => {}
 | fvar x => {x}
 | abs e1 => e1.fv
 | app l r => l.fv ∪ r.fv
 
 /-- Locally closed terms. -/
-inductive Term.LC : Term Var → Prop
+@[aesop safe (rule_sets := [LambdaCalculus.LocallyNameless.ruleSet]) [constructors]]
+inductive LC : Term Var → Prop
 | fvar (x)  : LC (fvar x)
 | abs (L : Finset Var) (e : Term Var) : (∀ x : Var, x ∉ L → LC (e ^ fvar x)) → LC (abs e)
 | app {l r} : l.LC → r.LC → LC (app l r)
