Cslib/Utils/Relation.lean
@@ -1,9 +1,44 @@
 /-
 Copyright (c) 2025 Thomas Waring. All rights reserved.
 Released under Apache 2.0 license as described in the file LICENSE.
-Authors: Thomas Waring
+Authors: Thomas Waring, Chris Henson
 -/
 import Mathlib.Logic.Relation
+
+universe u
+
+variable {α : Type u} {R R' : α → α → Prop}
+
+/-- A relation has the diamond property when all reductions with a common origin are joinable -/
+abbrev Diamond (R : α → α → Prop) := ∀ {A B C : α}, R A B → R A C → (∃ D, R B D ∧ R C D)
+
+/-- A relation is confluent when its reflexive transitive closure has the diamond property. -/
+abbrev Confluence (R : α → α → Prop) := Diamond (Relation.ReflTransGen R)
+
+/-- Extending a multistep reduction by a single step preserves multi-joinability. -/
+lemma Relation.ReflTransGen.diamond_extend (h : Diamond R) : 
+  Relation.ReflTransGen R A B → 
+  R A C → 
+  ∃ D, Relation.ReflTransGen R B D ∧ Relation.ReflTransGen R C D := by
+  intros AB _
+  revert C
+  induction AB using Relation.ReflTransGen.head_induction_on <;> intros C AC
+  case refl => exact ⟨C, ⟨single AC, by rfl⟩⟩
+  case head A'_C' _ ih =>
+    obtain ⟨D, ⟨CD, C'_D⟩⟩ := h AC A'_C'
+    obtain ⟨D', ⟨B_D', D_D'⟩⟩ := ih C'_D
+    exact ⟨D', ⟨B_D', head CD D_D'⟩⟩
+
+/-- The diamond property implies confluence. -/
+theorem Relation.ReflTransGen.diamond_confluence (h : Diamond R) : Confluence R := by
+  intros A B C AB BC
+  revert C
+  induction AB using Relation.ReflTransGen.head_induction_on <;> intros C BC
+  case refl => exists C
+  case head _ _ A'_C' _ ih =>
+    obtain ⟨D, ⟨CD, C'_D⟩⟩ := diamond_extend h BC A'_C'
+    obtain ⟨D', ⟨B_D', D_D'⟩⟩ := ih C'_D
+    exact ⟨D', ⟨B_D', trans CD D_D'⟩⟩
 
 -- not sure why this doesn't compile as an "instance" but oh well
 def trans_of_subrelation {α : Type _} (s s' r : α → α → Prop) (hr : Transitive r)
