Cslib/Computability/LambdaCalculus/Untyped/LocallyNameless/AesopRuleset.lean
@@ -1,0 +1,3 @@
+import Aesop
+
+declare_aesop_rule_sets [LambdaCalculus.LocallyNameless.ruleSet] (default := true)
