Cslib/Computability/LambdaCalculus/Untyped/LocallyNameless/FullBeta.lean
@@ -1,0 +1,122 @@
+/-
+Copyright (c) 2025 Chris Henson. All rights reserved.
+Released under Apache 2.0 license as described in the file LICENSE.
+Authors: Chris Henson
+-/
+
+import Cslib.Computability.LambdaCalculus.Untyped.LocallyNameless.Basic
+import Cslib.Computability.LambdaCalculus.Untyped.LocallyNameless.Properties
+import Cslib.Semantics.ReductionSystem.Basic
+
+/-! # β-reduction for the λ-calculus
+
+## References
+
+* [A. Chargueraud, *The Locally Nameless Representation*] [Chargueraud2012]
+* See also https://www.cis.upenn.edu/~plclub/popl08-tutorial/code/, from which
+  this is partially adapted
+
+-/
+
+universe u
+
+variable {Var : Type u} 
+
+namespace LambdaCalculus.LocallyNameless.Term
+
+/-- A single β-reduction step. -/
+@[reduction_sys fullBetaRs "βᶠ"]
+inductive FullBeta : Term Var → Term Var → Prop
+/-- Reduce an application to a lambda term. -/
+| beta : LC (abs M)→ LC N → FullBeta (app (abs M) N) (M ^ N)
+/-- Left congruence rule for application. -/
+| appL: LC Z → FullBeta M N → FullBeta (app Z M) (app Z N)
+/-- Right congruence rule for application. -/
+| appR : LC Z → FullBeta M N → FullBeta (app M Z) (app N Z)
+/-- Congruence rule for lambda terms. -/
+| abs (xs : Finset Var) : (∀ x ∉ xs, FullBeta (M ^ fvar x) (N ^ fvar x)) → FullBeta (abs M) (abs N) 
+
+namespace FullBeta
+
+variable {M M' N N' : Term Var}
+
+/-- The left side of a reduction is locally closed. -/
+lemma step_lc_l (step : M ⭢βᶠ M') : LC M := by
+  induction step <;> constructor
+  all_goals assumption
+
+/-- Left congruence rule for application in multiple reduction.-/
+theorem redex_app_l_cong : (M ↠βᶠ M') → LC N → (app M N ↠βᶠ app M' N) := by
+  intros redex lc_N 
+  induction' redex
+  case refl => rfl
+  case tail ih r => exact Relation.ReflTransGen.tail r (appR lc_N ih)
+
+/-- Right congruence rule for application in multiple reduction.-/
+theorem redex_app_r_cong : (M ↠βᶠ M') → LC N → (app N M ↠βᶠ app N M') := by
+  intros redex lc_N 
+  induction' redex
+  case refl => rfl
+  case tail ih r => exact Relation.ReflTransGen.tail r (appL lc_N ih)
+
+variable [HasFresh Var] [DecidableEq Var]
+
+/-- The right side of a reduction is locally closed. -/
+lemma step_lc_r (step : M ⭢βᶠ M') : LC M' := by
+  induction step
+  case beta => apply beta_lc <;> assumption
+  all_goals try constructor <;> assumption 
+
+/-- Substitution respects a single reduction step. -/
+lemma redex_subst_cong (s s' : Term Var) (x y : Var) : (s ⭢βᶠ s') → (s [ x := fvar y ]) ⭢βᶠ (s' [ x := fvar y ]) := by
+  intros step
+  induction step
+  case appL ih => exact appL (subst_lc (by assumption) (by constructor)) ih 
+  case appR ih => exact appR (subst_lc (by assumption) (by constructor)) ih  
+  case beta m n abs_lc n_lc => 
+    cases abs_lc with | abs xs _ mem =>
+      simp only [open']
+      rw [subst_open x (fvar y) 0 n m (by constructor)]
+      refine beta ?_ (subst_lc n_lc (by constructor))
+      exact subst_lc (LC.abs xs m mem) (LC.fvar y)
+  case abs m' m xs mem ih => 
+    apply abs ({x} ∪ xs)
+    intros z z_mem
+    simp only [open']
+    rw [
+      subst_def, subst_def,
+      ←subst_fresh x (fvar z) (fvar y), ←subst_open x (fvar y) 0 (fvar z) m (by constructor),
+      subst_fresh x (fvar z) (fvar y), ←subst_fresh x (fvar z) (fvar y),
+      ←subst_open x (fvar y) 0 (fvar z) m' (by constructor), subst_fresh x (fvar z) (fvar y)
+    ]
+    apply ih
+    all_goals aesop
+
+/-- Abstracting then closing preserves a single reduction. -/
+lemma step_abs_close {x : Var} : (M ⭢βᶠ M') → (M⟦0 ↜ x⟧.abs ⭢βᶠ M'⟦0 ↜ x⟧.abs) := by
+  intros step
+  apply abs ∅
+  intros y _
+  simp only [open']
+  repeat rw [open_close_to_subst]
+  exact redex_subst_cong M M' x y step
+  exact step_lc_r step
+  exact step_lc_l step
+
+/-- Abstracting then closing preserves multiple reductions. -/
+lemma redex_abs_close {x : Var} : (M ↠βᶠ M') → (M⟦0 ↜ x⟧.abs ↠βᶠ M'⟦0 ↜ x⟧.abs) :=  by
+  intros step
+  induction step using Relation.ReflTransGen.trans_induction_on
+  case ih₁ => rfl
+  case ih₂ ih => exact Relation.ReflTransGen.single (step_abs_close ih)
+  case ih₃ l r => trans; exact l; exact r
+
+/-- Multiple reduction of opening implies multiple reduction of abstraction. -/
+theorem redex_abs_cong (xs : Finset Var) : (∀ x ∉ xs, (M ^ fvar x) ↠βᶠ (M' ^ fvar x)) → M.abs ↠βᶠ M'.abs := by
+  intros mem
+  have ⟨fresh, union⟩ := fresh_exists (xs ∪ M.fv ∪ M'.fv)
+  simp only [Finset.union_assoc, Finset.mem_union, not_or] at union
+  obtain ⟨_, _, _⟩ := union
+  rw [←open_close fresh M 0 ?_, ←open_close fresh M' 0 ?_]
+  refine redex_abs_close (mem fresh ?_)
+  all_goals assumption
