Cslib/Computability/LambdaCalculus/Untyped/LocallyNameless/FullBetaConfluence.lean
@@ -1,0 +1,254 @@
+/-
+Copyright (c) 2025 Chris Henson. All rights reserved.
+Released under Apache 2.0 license as described in the file LICENSE.
+Authors: Chris Henson
+-/
+
+import Cslib.Computability.LambdaCalculus.Untyped.LocallyNameless.Basic
+import Cslib.Computability.LambdaCalculus.Untyped.LocallyNameless.Properties
+import Cslib.Computability.LambdaCalculus.Untyped.LocallyNameless.FullBeta
+import Cslib.Utils.Relation
+
+/-! # β-confluence for the λ-calculus -/
+
+universe u
+
+variable {Var : Type u} 
+
+namespace LambdaCalculus.LocallyNameless.Term
+
+/-- A parallel β-reduction step. -/
+@[aesop safe (rule_sets := [LambdaCalculus.LocallyNameless.ruleSet]) [constructors], reduction_sys paraRs "ₚ"]
+inductive Parallel : Term Var → Term Var → Prop
+/-- Free variables parallel step to themselves. -/
+| fvar (x : Var) : Parallel (fvar x) (fvar x)
+/-- A parallel left and right congruence rule for application. -/
+| app : Parallel L L' → Parallel M M' → Parallel (app L M) (app L' M')
+/-- Congruence rule for lambda terms. -/
+| abs (xs : Finset Var) : (∀ x ∉ xs, Parallel (m ^ fvar x) (m' ^ fvar x)) → Parallel (abs m) (abs m')
+/-- A parallel β-reduction. -/
+| beta (xs : Finset Var) : 
+    (∀ x ∉ xs, Parallel (m ^ fvar x) (m' ^ fvar x) ) →
+    Parallel n n' → 
+    Parallel (app (abs m) n) (m' ^ n')
+
+-- TODO: I think this could be generated along with `para_rs`
+lemma para_rs_Red_eq {α} : (@paraRs α).Red = Parallel := by rfl
+
+variable {M M' N N' : Term Var}
+
+/-- The left side of a parallel reduction is locally closed. -/
+@[aesop unsafe (rule_sets := [LambdaCalculus.LocallyNameless.ruleSet])]
+lemma para_lc_l (step : M ⭢ₚ N) : LC M  := by
+  induction step
+  case abs _ _ xs _ ih => exact LC.abs xs _ ih
+  case beta => refine LC.app (LC.abs ?_ _ ?_) ?_ <;> assumption
+  all_goals constructor <;> assumption
+
+variable [HasFresh Var] [DecidableEq Var]
+
+/-- The right side of a parallel reduction is locally closed. -/
+@[aesop unsafe (rule_sets := [LambdaCalculus.LocallyNameless.ruleSet])]
+lemma para_lc_r (step : M ⭢ₚ N) : LC N := by
+  induction step
+  case abs _ _ xs _ ih => exact LC.abs xs _ ih
+  case beta => refine beta_lc (LC.abs ?_ _ ?_) ?_ <;> assumption
+  all_goals constructor <;> assumption
+
+/-- Parallel reduction is reflexive for locally closed terms. -/
+@[aesop safe (rule_sets := [LambdaCalculus.LocallyNameless.ruleSet])]
+def Parallel.lc_refl (M : Term Var) : LC M → M ⭢ₚ M := by
+  intros lc
+  induction lc
+  all_goals constructor <;> assumption
+
+-- TODO: better ways to handle this?
+-- The problem is that sometimes when we apply a theorem we get out of our notation, so aesop can't
+-- see they are the same, including constructors.
+@[aesop safe (rule_sets := [LambdaCalculus.LocallyNameless.ruleSet])]
+def Parallel.lc_refl' (M : Term Var) : LC M → Parallel M M := Parallel.lc_refl M
+
+omit [HasFresh Var] [DecidableEq Var] in
+/-- A single β-reduction implies a single parallel reduction. -/
+lemma step_to_para (step : M ⭢βᶠ N) : (M ⭢ₚ N) := by
+  induction step <;> simp only [para_rs_Red_eq]
+  case beta _ abs_lc _ => cases abs_lc with | abs xs _ => 
+    apply Parallel.beta xs <;> intros <;> apply Parallel.lc_refl <;> aesop
+  all_goals aesop (config := {enableSimp := false})
+
+open FullBeta in
+/-- A single parallel reduction implies a multiple β-reduction. -/
+lemma para_to_redex (para : M ⭢ₚ N) : (M ↠βᶠ N) := by
+  induction para
+  case fvar => constructor
+  case app _ _ _ _ l_para m_para redex_l redex_m =>
+    trans
+    exact redex_app_l_cong redex_l (para_lc_l m_para)
+    exact redex_app_r_cong redex_m (para_lc_r l_para)
+  case abs t t' xs _ ih =>
+    apply redex_abs_cong xs
+    intros x mem
+    exact ih x mem
+  case beta m m' n n' xs para_ih para_n redex_ih redex_n =>
+    have m'_abs_lc : LC m'.abs := by
+      apply LC.abs xs
+      intros _ mem
+      exact para_lc_r (para_ih _ mem)
+    calc
+      m.abs.app n ↠βᶠ m'.abs.app n  := redex_app_l_cong (redex_abs_cong xs (λ _ mem ↦ redex_ih _ mem)) (para_lc_l para_n)
+      _           ↠βᶠ m'.abs.app n' := redex_app_r_cong redex_n m'_abs_lc
+      _           ⭢βᶠ m' ^ n'       := beta m'_abs_lc (para_lc_r para_n)
+
+/-- Multiple parallel reduction is equivalent to multiple β-reduction. -/
+theorem parachain_iff_redex : (M ↠ₚ N) ↔ (M ↠βᶠ N) := by
+  refine Iff.intro ?chain_to_redex ?redex_to_chain <;> intros h <;> induction' h <;> try rfl
+  case redex_to_chain.tail redex chain => exact Relation.ReflTransGen.tail chain (step_to_para redex)
+  case chain_to_redex.tail para  redex => exact Relation.ReflTransGen.trans redex (para_to_redex para)
+
+/-- Parallel reduction respects substitution. -/
+lemma para_subst (x : Var) : (M ⭢ₚ M') → (N ⭢ₚ N') → (M[x := N] ⭢ₚ M'[x := N']) := by
+  intros pm pn
+  induction pm
+  case fvar => aesop
+  case beta _ _ _ _ xs _ _ ih _ => 
+    simp only [open']
+    rw [subst_open _ _ _ _ _ (para_lc_r pn)]
+    apply Parallel.beta (xs ∪ {x})
+    intros y ymem
+    simp only [Finset.mem_union, Finset.mem_singleton, not_or] at ymem
+    push_neg at ymem
+    rw [
+      subst_def, 
+      subst_open_var _ _ _ _ _ (para_lc_r pn), 
+      subst_open_var _ _ _ _ _ (para_lc_l pn)
+    ]
+    apply ih
+    all_goals aesop
+  case app => constructor <;> assumption
+  case abs u u' xs mem ih => 
+    apply Parallel.abs (xs ∪ {x})
+    intros y ymem
+    simp only [Finset.mem_union, Finset.mem_singleton, not_or] at ymem
+    repeat rw [subst_def]
+    rw [subst_open_var _ _ _ _ ?_ (para_lc_l pn), subst_open_var _ _ _ _ ?_ (para_lc_r pn)]
+    push_neg at ymem
+    apply ih
+    all_goals aesop
+
+/-- Parallel substitution respects closing and opening. -/
+lemma para_open_close (x y z) : 
+  (M ⭢ₚ M') → 
+  y ∉ (M.fv ∪ M'.fv ∪ {x}) → 
+  M⟦z ↜ x⟧⟦z ↝ fvar y⟧ ⭢ₚ M'⟦z ↜ x⟧⟦z ↝ fvar y⟧ 
+  := by
+  intros para vars
+  simp only [Finset.union_assoc, Finset.mem_union, Finset.mem_singleton, not_or] at vars
+  rw [open_close_to_subst, open_close_to_subst] 
+  apply para_subst
+  exact para
+  constructor
+  exact para_lc_r para
+  exact para_lc_l para
+
+/-- Parallel substitution respects fresh opening. -/
+lemma para_open_out (L : Finset Var) :
+    (∀ x, x ∉ L → (M ^ fvar x) ⭢ₚ (N ^ fvar x))
+    → (M' ⭢ₚ N') → (M ^ M') ⭢ₚ (N ^ N') := by
+    intros mem para
+    let ⟨x, qx⟩ := fresh_exists (L ∪ N.fv ∪ M.fv)
+    simp only [Finset.union_assoc, Finset.mem_union, not_or] at qx
+    obtain ⟨q1, q2, q3⟩ := qx
+    rw [subst_intro x M' _ q3 (para_lc_l para), subst_intro x N' _ q2 (para_lc_r para)]
+    exact para_subst x (mem x q1) para
+
+-- TODO: the Takahashi translation would be a much nicer and shorter proof, but I had difficultly
+-- writing it for locally nameless terms.
+
+-- adapted from https://github.com/ElifUskuplu/Stlc_deBruijn/blob/main/Stlc/confluence.lean
+/-- Parallel reduction has the diamond property. -/
+theorem para_diamond : Diamond (@Parallel Var) := by
+  intros t t1 t2 tpt1
+  revert t2
+  induction tpt1 <;> intros t2 tpt2
+  case fvar x => exact ⟨t2, by aesop⟩
+  case abs s1 s2' xs mem ih => 
+    cases tpt2
+    case abs t2' xs' mem' =>
+      have ⟨x, qx⟩ := fresh_exists (xs ∪ xs' ∪ t2'.fv ∪ s2'.fv)
+      simp only [Finset.union_assoc, Finset.mem_union, not_or] at qx
+      have ⟨q1, q2, q3, q4⟩ := qx
+      have ⟨t', qt'_l, qt'_r⟩ := ih x q1 (mem' _ q2)
+      exists abs (t' ^* x)
+      constructor 
+      <;> [let z := s2'; let z := t2']
+      <;> apply Parallel.abs ((z ^ fvar x).fv ∪ t'.fv ∪ {x})
+      <;> intros y qy <;> simp only [open', close]
+      <;> [rw [←open_close x _ 0 q4]; rw [←open_close x _ 0 q3]] 
+      <;> refine para_open_close x y 0 ?_ qy <;> [exact qt'_l; exact qt'_r]
+  case beta s1 s1' s2 s2' xs mem ps ih1 ih2 => 
+    cases tpt2
+    case app u2 u2' s1pu2 s2pu2' => 
+      cases s1pu2
+      case abs s1'' xs' mem' =>
+        have ⟨x, qx⟩ := fresh_exists (xs ∪ xs' ∪ s1''.fv ∪ s1'.fv)
+        simp only [Finset.union_assoc, Finset.mem_union, not_or] at qx
+        obtain ⟨q1, q2, q3, q4⟩ := qx
+        have ⟨t', qt'_l, qt'_r⟩ := ih2 s2pu2'
+        have ⟨t'', qt''_l, qt''_r⟩ := @ih1 x q1 _ (mem' _ q2)
+        exists (t'' ^* x) ^ t'
+        constructor
+        · rw [subst_intro x s2' _ q4 (para_lc_l qt'_l), 
+              subst_intro x t' _ (close_var_not_fvar x t'') (para_lc_r qt'_l)]
+          simp only [open', close]
+          rw [close_open _ _ _ (para_lc_r qt''_l)]
+          exact para_subst x qt''_l qt'_l
+        · apply Parallel.beta ((s1'' ^ fvar x).fv ∪ t''.fv ∪ {x})
+          intros y qy
+          rw [←open_close x s1'' 0]
+          apply para_open_close
+          all_goals aesop
+    case beta u1' u2' xs' mem' s2pu2' => 
+      have ⟨x, qx⟩ := fresh_exists (xs ∪ xs' ∪ u1'.fv ∪ s1'.fv ∪ s2'.fv ∪ u2'.fv)
+      simp only [Finset.union_assoc, Finset.mem_union, not_or] at qx
+      have ⟨q1, q2, q3, q4, q5, q6⟩ := qx
+      have ⟨t', qt'_l, qt'_r⟩ := ih2 s2pu2'
+      have ⟨t'', qt''_l, qt''_r⟩ := @ih1 x q1 _ (mem' _ q2)
+      rw [subst_intro x u2' u1' _ (para_lc_l qt'_r), subst_intro x s2' s1' _ (para_lc_l qt'_l)]
+      exists t'' [x := t']
+      exact ⟨para_subst x qt''_l qt'_l, para_subst x qt''_r qt'_r⟩
+      all_goals aesop
+  case app s1 s1' s2 s2' s1ps1' _ ih1 ih2  =>
+    cases tpt2
+    case app u1 u2' s1 s2 =>
+      have ⟨l, _, _⟩ := ih1 s1
+      have ⟨r, _, _⟩ := ih2 s2
+      exact ⟨app l r, by aesop⟩
+    case beta t1' u1' u2' xs mem s2pu2' => 
+      cases s1ps1'
+      case abs s1'' xs' mem' =>
+        have ⟨x, qx⟩ := fresh_exists (xs ∪ xs' ∪ s1''.fv ∪ u1'.fv)
+        simp only [Finset.union_assoc, Finset.mem_union, not_or] at qx
+        obtain ⟨q1, q2, q3, q4⟩ := qx
+        have ⟨t', qt'_l, qt'_r⟩ := ih2 s2pu2'
+        have ⟨t'', qt''_l, qt''_r⟩ := @ih1 (abs u1') (Parallel.abs xs mem)
+        cases qt''_l
+        next w1 xs'' mem'' =>
+        cases qt''_r
+        case abs xs''' mem''' =>
+          exists w1 ^ t'
+          constructor
+          · aesop (config := {enableSimp := false})
+          · exact para_open_out xs''' mem''' qt'_r
+
+/-- Parallel reduction is confluent. -/
+theorem para_confluence : Confluence (@Parallel Var) := 
+  Relation.ReflTransGen.diamond_confluence para_diamond
+
+/-- β-reduction is confluent. -/
+theorem confluence_beta : Confluence (@FullBeta Var) := by
+  simp only [Confluence]
+  have eq : Relation.ReflTransGen (@Parallel Var) = Relation.ReflTransGen (@FullBeta Var) := by
+    ext
+    exact parachain_iff_redex
+  rw [←eq]
+  exact @para_confluence Var _ _
