Cslib/Computability/LambdaCalculus/Untyped/LocallyNameless/Properties.lean
@@ -12,44 +12,43 @@ variable {Var : Type u}
 
 namespace LambdaCalculus.LocallyNameless.Term
 
+lemma open_app_inj : app l r = (app l r)⟦i ↝ s⟧ ↔ l = l⟦i ↝ s⟧ ∧ r = r⟦i ↝ s⟧ := by
+  simp [openRec]
+
+lemma open_abs_inj : M.abs = M⟦i + 1 ↝ s⟧.abs ↔ M = M⟦i + 1 ↝ s⟧ := by
+  simp
+
 /-- An opening appearing in both sides of an equality of terms can be removed. -/
 lemma open_lc_aux (e : Term Var) : ∀ (j v i u),
-  i ≠ j ->
-  e ⟦j ↝ v⟧ = (e ⟦j ↝ v⟧) ⟦i ↝ u⟧ ->
+  i ≠ j →
+  e ⟦j ↝ v⟧ = (e ⟦j ↝ v⟧) ⟦i ↝ u⟧ →
   e = e ⟦i ↝ u⟧ := by
-  induction' e 
-  <;> intros j v i u neq h 
-  <;> simp only [openRec, app.injEq, abs.injEq] at *
-  case bvar => aesop
-  case app ih_l ih_r => 
-    obtain ⟨hl, hr⟩ := h
+  induction' e <;> intros j v i u neq h 
+  case app l r ih_l ih_r => 
+    obtain ⟨hl, hr⟩ := open_app_inj.mp h
+    simp only [open_app_inj]
     exact ⟨ih_l j v i u neq hl, ih_r j v i u neq hr⟩
-  case abs ih => exact ih (j+1) v (i+1) u (by aesop) h
+  case abs ih =>
+    simp only [openRec_abs, open_abs_inj] at *
+    exact ih (j+1) v (i+1) u (by aesop) h
+  all_goals aesop
 
 /-- Opening is associative for nonclashing free variables. -/
 lemma swap_open_fvars (k n : ℕ) (x y : Var) (m : Term Var) : 
     k ≠ n → x ≠ y → m⟦n ↝ fvar y⟧⟦k ↝ fvar x⟧ = m⟦k ↝ fvar x⟧⟦n ↝ fvar y⟧ := by
   revert k n
-  induction' m <;> intros k n ne_kn ne_xy <;> simp only [openRec, app.injEq, abs.injEq]
-  case bvar n' => aesop
-  case abs ih => apply ih <;> aesop
-  case app => aesop
+  induction' m <;> aesop
 
 variable [DecidableEq Var]
 
 /-- Substitution of a free variable not present in a term leaves it unchanged. -/
 theorem subst_fresh (x : Var) (t sub : Term Var) : x ∉ t.fv → (t [x := sub]) = t := by
-  induction t <;> intros <;> aesop
+  induction t <;> aesop
 
 /- Opening and closing are inverses. -/
 lemma open_close (x : Var) (t : Term Var) (k : ℕ) : x ∉ t.fv → t⟦k ↝ fvar x⟧⟦k ↜ x⟧ = t := by
-  intros mem
   revert k
-  induction t <;> intros k <;> simp only [openRec, closeRec, app.injEq, abs.injEq]
-  case bvar n => split <;> simp_all
-  case abs t ih => exact ih mem (k + 1)
-  case app l r ih_l ih_r => refine ⟨ih_l ?_ k, ih_r ?_ k⟩ <;> aesop
-  all_goals aesop
+  induction t <;> aesop
 
 /-- Opening is injective. -/
 lemma open_injective (x : Var) (M M' : Term Var) : x ∉ M.fv → x ∉ M'.fv → M ^ fvar x = M' ^ fvar x → M = M' := by
@@ -61,49 +60,27 @@ lemma open_injective (x : Var) (M M' : Term Var) : x ∉ M.fv → x ∉ M'.fv �
 lemma swap_open_fvar_close (k n: ℕ) (x y : Var) (m : Term Var) : 
     k ≠ n → x ≠ y → m⟦n ↝ fvar y⟧⟦k ↜ x⟧ = m⟦k ↜ x⟧⟦n ↝ fvar y⟧ := by
   revert k n
-  induction' m 
-  <;> intros k n ne_kn ne_xy 
-  <;> simp only [openRec, closeRec, app.injEq, abs.injEq]
-  case bvar n'  => split <;> aesop
-  case fvar x'  => split <;> aesop
-  case abs ih => apply ih <;> aesop
-  case app => aesop
+  induction' m <;> aesop
 
 /-- Closing preserves free variables. -/
 lemma close_preserve_not_fvar {k x y} (m : Term Var) : x ∉ m.fv → x ∉ (m⟦k ↜ y⟧).fv := by
-  intros mem
   revert k
-  induction m <;> intros k <;> simp only [closeRec]
-  case fvar y' => split <;> aesop
-  case abs ih => exact ih mem
-  all_goals aesop
+  induction m <;> aesop
 
 /-- Opening to a fresh free variable preserves free variables. -/
 lemma open_fresh_preserve_not_fvar {k x y} (m : Term Var) : x ∉ m.fv → x ≠ y → x ∉ (m⟦k ↝ fvar y⟧).fv := by
-  intros mem neq
   revert k
-  induction m <;> intros k <;> simp only [openRec]
-  case bvar n'  => split <;> aesop
-  case fvar => aesop
-  case abs ih => exact ih mem
-  all_goals aesop
+  induction m <;> aesop
 
 /-- Substitution preserves free variables. -/
 lemma subst_preserve_not_fvar {x y : Var} (m n : Term Var) : x ∉ m.fv ∪ n.fv → x ∉ (m [y := n]).fv := by
-  intros mem
-  simp only [Finset.mem_union, not_or] at mem
-  induction m <;> simp only [instHasSubstitutionTerm, subst]
-  case fvar y' => split <;> simp only [fv, Finset.mem_singleton, mem] <;> aesop
-  case abs ih => exact ih mem
+  induction m
   all_goals aesop
 
 /-- Closing removes a free variable. -/
 lemma close_var_not_fvar_rec (x) (k) (t : Term Var) : x ∉ (t⟦k ↜ x⟧).fv := by
   revert k
-  induction t <;> intros k <;> simp only [closeRec]
-  case fvar x' => split <;> simp_all
-  case abs ih => exact ih (k + 1)
-  all_goals aesop
+  induction t <;> aesop
 
 /-- Specializes `close_var_not_fvar_rec` to first closing. -/
 lemma close_var_not_fvar (x) (t : Term Var) : x ∉ (t ^* x).fv := close_var_not_fvar_rec x 0 t
@@ -112,55 +89,47 @@ variable [HasFresh Var]
 
 omit [DecidableEq Var] in
 /-- A locally closed term is unchanged by opening. -/
+@[aesop safe (rule_sets := [LambdaCalculus.LocallyNameless.ruleSet])]
 lemma open_lc (k t) (e : Term Var) : e.LC → e = e⟦k ↝ t⟧ := by
   intros e_lc
   revert k
-  induction e_lc <;> intros k <;> simp only [openRec, app.injEq, abs.injEq]
-  case app => aesop
-  case abs xs e _ ih => refine open_lc_aux e 0 (fvar (fresh xs)) (k+1) t ?_ ?_ <;> aesop
+  induction e_lc
+  case abs xs e _ ih => 
+    intros k
+    simp only [openRec_abs, abs.injEq]
+    refine open_lc_aux e 0 (fvar (fresh xs)) (k+1) t ?_ ?_ <;> aesop
+  all_goals aesop
 
 /-- Substitution of a locally closed term distributes with opening. -/
 lemma subst_open (x : Var) (t : Term Var) (k : ℕ) (u e) :
   LC t → 
   (e ⟦ k ↝ u ⟧) [ x := t ] = (e [ x := t ]) ⟦k ↝  u [ x := t ]⟧ := by
   revert k
-  induction' e 
-  <;> intros k t_lv 
-  <;> simp only [openRec, instHasSubstitutionTerm, subst, app.injEq, abs.injEq]
-  case bvar k' => aesop
-  case fvar x' => 
-    split <;> simp_all
-    exact open_lc k (u[x':=t]) t t_lv
-  case abs ih => exact ih (k + 1) t_lv
-  case app ih_l ih_r => exact ⟨ih_l k t_lv, ih_r k t_lv⟩
+  induction' e <;> aesop
 
 /-- Specialize `subst_open` to the first opening. -/
 theorem subst_open_var (x y : Var) (u e : Term Var) : y ≠ x → LC u → (e [y := u]) ^ fvar x = (e ^ fvar x) [y := u] := by
   intros neq u_lc
-  have := subst_open y u 0 (fvar x) e u_lc
+  have h : (e ^ fvar x)[y:=u] = e[y:=u] ^ (fvar x)[y:=u] := subst_open y u 0 (fvar x) e u_lc
   aesop
 
 /-- Substitution of locally closed terms is locally closed. -/
 theorem subst_lc {x : Var} {e u : Term Var} : LC e → LC u → LC (e [x := u]) := by
   intros lc_e lc_u
-  induction lc_e <;> simp only [instHasSubstitutionTerm, subst]
-  case fvar => split <;> [assumption; constructor] 
-  case app ih_l ih_r => exact LC.app ih_l ih_r
+  induction lc_e 
   case abs xs e _ ih =>
     refine LC.abs ({x} ∪ xs) _ (?_ : ∀ y ∉ {x} ∪ xs, (e[x := u] ^ fvar y).LC)
     intros y mem
     rw [subst_open_var y x u e ?_ lc_u]
-    apply ih
     all_goals aesop
+  all_goals aesop
 
 /-- Opening to a term `t` is equivalent to opening to a free variable and substituting it for `t`. -/
 lemma subst_intro (x : Var) (t e : Term Var) : x ∉ e.fv → LC t → e ^ t = (e ^ fvar x) [ x := t ] := by
   intros mem t_lc
   simp only [open']
-  rw [subst_open x t 0 (fvar x) e t_lc]
-  have s := subst_fresh _ _ t mem
-  simp only [instHasSubstitutionTerm, subst, ↓reduceIte] at *
-  rw [s]
+  rw [subst_open x t 0 (fvar x) e t_lc, subst_fresh _ _ t mem]
+  aesop
 
 /-- Opening of locally closed terms is locally closed. -/
 theorem beta_lc {M N : Term Var} : LC (abs M) → LC N → LC (M ^ N) := by
@@ -174,23 +143,20 @@ theorem beta_lc {M N : Term Var} : LC (abs M) → LC N → LC (M ^ N) := by
     rw [subst_intro y N M]
     apply subst_lc
     apply mem
-    all_goals aesop        
+    all_goals aesop
 
 /-- Opening then closing is equivalent to substitution. -/
 lemma open_close_to_subst (m : Term Var) (x y : Var) (k : ℕ) : LC m → m ⟦k ↜ x⟧⟦k ↝ fvar y⟧ = m [x := fvar y] := by
   intros m_lc
   revert k
   induction' m_lc 
-  <;> intros k 
-  <;> simp only [closeRec, openRec, instHasSubstitutionTerm, subst, abs.injEq, app.injEq]
-  case fvar x' => split <;> simp
-  case app ih_l ih_r => exact ⟨ih_l _, ih_r _⟩
   case abs xs t x_mem ih =>
+    intros k
     have ⟨x', x'_mem⟩ := fresh_exists ({x} ∪ {y} ∪ t.fv ∪ xs)
     have s := subst_open_var x' x (fvar y) t ?_ (by constructor)
-    simp only [open', Finset.union_assoc, Finset.mem_union, Finset.mem_singleton, not_or] at *
-    rw [←open_close x' (t⟦k+1 ↜ x⟧⟦k+1 ↝ fvar y⟧) 0 ?f₁, ←open_close x' (t.subst x (fvar y)) 0 ?f₂]
-    simp [instHasSubstitutionTerm] at s
+    simp only [closeRec_abs, openRec_abs, subst_abs]
+    rw [←open_close x' (t⟦k+1 ↜ x⟧⟦k+1 ↝ fvar y⟧) 0 ?f₁, ←open_close x' (t[x := fvar y]) 0 ?f₂]
+    simp only [open'] at *
     rw [swap_open_fvars, ←swap_open_fvar_close, s, ih]
     case f₁ =>
       apply open_fresh_preserve_not_fvar
@@ -200,14 +166,16 @@ lemma open_close_to_subst (m : Term Var) (x y : Var) (k : ℕ) : LC m → m ⟦k
       apply subst_preserve_not_fvar
       aesop
     all_goals aesop
+  all_goals aesop
 
 /-- Closing and opening are inverses. -/
 lemma close_open (x : Var) (t : Term Var) (k : ℕ) : LC t → t⟦k ↜ x⟧⟦k ↝ fvar x⟧ = t := by
   intros lc_t
   revert k
-  induction lc_t <;> intros k <;> simp only [closeRec, openRec, abs.injEq, app.injEq]
-  case fvar x' => split <;> simp_all
+  induction lc_t
   case abs xs t t_open_lc ih => 
+    intros k
+    simp only [closeRec_abs, openRec_abs, abs.injEq]
     have ⟨y, hy⟩ := fresh_exists (xs ∪ t.fv ∪ (t⟦k + 1 ↜ x⟧⟦k + 1 ↝ fvar x⟧).fv ∪ {x})
     simp only [Finset.union_assoc, Finset.mem_union, Finset.mem_singleton, not_or] at hy
     obtain ⟨q1, q2, q3, q4⟩ := hy
@@ -216,4 +184,4 @@ lemma close_open (x : Var) (t : Term Var) (k : ℕ) : LC t → t⟦k ↜ x⟧⟦
     simp only [open']
     rw [swap_open_fvar_close, swap_open_fvars]
     all_goals aesop
-  case app => aesop
+  all_goals aesop
